fstar-helpers/fstar-bitvec/Tactics.Seq.fst
@@ -1,0 +1,49 @@
+module Tactics.Seq
+
+open Core
+module L = FStar.List.Tot
+open FStar.Tactics.V2
+open FStar.Tactics.V2.SyntaxHelpers
+open FStar.Class.Printable
+open FStar.Mul
+open FStar.Option
+
+open Tactics.Utils
+open Tactics.Pow2
+
+let rw_seq_index_list #t (l: list t) i
+    : Lemma (Seq.Base.index (Seq.Base.seq_of_list l) i == FStar.List.Tot.index l i) 
+    = ()
+
+private let unfold_index_lemma (#a: Type) (l: list a) (i:nat{i < List.Tot.length l})
+  : Lemma (  FStar.List.Tot.index #a l i 
+          == Pervasives.norm [iota; primops] (let hd::tl = l in
+    if i = 0 then hd else List.Tot.index tl (i - 1)))
+  = ()
+
+private exception DoRefl
+private exception StopNormIndex
+let norm_list_index (): Tac unit =
+  let _ = repeat (fun _ ->
+    lset "found" false;
+    pointwise (fun _ ->
+      (fun () ->
+         match let?# (t, _) = expect_lhs_eq_uvar () in
+               let?# (f, [typ, _; l, _; index, _]) = expect_app_n t 3 in
+               let?# () = expect_free_var f (`%FStar.List.Tot.index) in
+               let?# n = expect_int_literal index in
+               apply_lemma_rw (`unfold_index_lemma);
+               lset "found" true;
+               Some ()
+         with | Some () -> () | _ -> raise DoRefl
+      ) `or_else` trefl);
+    if lget "found" then () else raise StopNormIndex) in ()
+
+let _ = assert (L.index [1;2;3;4;5;6] 3 == 4) by (norm_list_index(); trefl ())
+
+let simplify_index_seq_of_list () = l_to_r [`rw_seq_index_list]
+
+let norm_index (): Tac unit
+  = norm_list_index ();
+    simplify_index_seq_of_list ()
+
