fstar-helpers/fstar-bitvec/Tactics.Utils.fst
@@ -1,0 +1,67 @@
+module Tactics.Utils
+
+open Core
+module L = FStar.List.Tot
+open FStar.Tactics.V2
+open FStar.Tactics.V2.SyntaxHelpers
+open FStar.Class.Printable
+open FStar.Mul
+open FStar.Option
+
+
+let (let?#) (x: option 'a) (f: 'a -> Tac (option 'b)): Tac (option 'b)
+  = match x with
+  | Some x -> f x
+  | None   -> None
+
+let ( let?? ) (x: bool) (f: unit -> Tac (option 'a)): Tac (option 'a)
+  = if x then f () else None
+
+let expect_int_literal (t: term): Tac (option int) =
+    match inspect_unascribe t with
+    | Tv_Const (C_Int n) -> Some n
+    | _ -> None
+
+let expect_fvar (t: term): Tac (option string) =
+    match t with
+    | Tv_UInst fv _
+    | Tv_FVar fv -> Some (implode_qn (inspect_fv fv))
+    | _ -> None
+
+let expect_free_var (t: term) (fv: string): Tac (option unit) =
+    let?# fv' = expect_fvar t in
+    if fv = fv' then Some () else None
+
+let expect_lhs_eq_rhs () = 
+    match FStar.Tactics.V2.Logic.cur_formula () with
+    | Comp (Eq typ) lhs rhs -> 
+      let typ = match typ with | None -> `_ | Some typ -> typ in
+      Some (lhs, rhs, typ)
+    | _ -> None
+
+let expect_lhs_eq_uvar () = 
+    match expect_lhs_eq_rhs () with
+    | Some (lhs, rhs, typ) -> 
+      ( match rhs with | Tv_Uvar _ _ -> Some (lhs, typ) | _ -> None )
+    | _ -> None
+
+let expect_app_n t n: Tac (option (term & (l: list _ {L.length l == n}))) =
+    let (head, args) = collect_app t in
+    if L.length args = n
+    then Some (head, args)
+    else None
+
+private exception ForceRevert
+let revert_if_none (f: unit -> Tac (option 'a)): Tac (option 'a)
+  = try match f () with Some x -> Some x 
+                      | None -> raise ForceRevert
+    with | ForceRevert -> None | e -> raise e
+
+/// Collects an application whose head is a free variable
+let collect_app_hd t: Tac (option (string & list argv))
+  = let (hd, args) = collect_app t in
+    let?# fv = expect_fvar hd in
+    Some (fv, args)
+
+let rec repeatWhile (f: unit -> Tac bool): Tac unit
+  = if f () then repeatWhile f
